# Completing the Square
*If you already know how to do this **efficiently**, you may skip.*

## Basic-How-To
**Goal:** You are tring to turn a trinomial into a completed square.

Take this equation for instance: $y=12x+2x^2+1$

We will try to get it here: $y=2(x+3)^2-17$

1. **Reorder the terms**
	* It will make things easier, I promise.
	* $y=2x^2+12x+1$

2. **Factor from the variable**
	* If there is a coefficient on the $x^2$, factor that number out from all other matching variables. In this case, we will factor $2$ from $2x^2$ and $12x$.
		* *Make sure to factor out the negative too!*
	* $y=2(x^2+6x)+1$

3. **Add & Subtract the constant**
	* Now its time to complete the square. To find the 3rd term, the constant, take the coefficent of the second term, divide by 2, then square it. 
	* $(\frac{6}{2})^2=9$
	* Now we have the constant, we can add it to the equation to create a perfect square! But we also need to subtract the same value to make the equation equal. We need to subtract the value we added **times** the number we factored with.
	* $y=2(x^2+6x+9)-9\times2+1$

4. **Simplify**
	* $2(x^2+6x+9)-17$
	* $2(x+3)^2-17$ <-- TADA :tada:

## Let's Practice
<!-- tabs:start -->

#### **Problem 1**
$y=49+x^2+14x$
* *$y=(x+7)^2$*

#### **Problem 2**
$y=x^2+6x+1$
* *$y=(x+3)^2-8$*

#### **Problem 3**
$y=3x^2+2x-3+4$
* *$y=3\left(x+\frac{1}{3}\right)^2+\frac{2}{3}$*

#### **Problem 4**
$y=2x^2+12x-8+4$
* *$y=2\left(x+3\right)^2-22$*

<!-- tabs:end -->